test: do no use unit in ac_expr.lean.
It is not necessary to define a unit element for the proof to go through.

tests/lean/run/ac_expr.lean
@@ -1,18 +1,24 @@
 import Std
 
-inductive Expr where
-  | var (i : Nat)
-  | op  (lhs rhs : Expr)
-  deriving Inhabited, Repr
+inductive Expr (maxVarId : Nat) : Type where
+  | var (i : Fin maxVarId)
+  | op  (lhs rhs : Expr maxVarId)
+  deriving Repr
 
-def List.getIdx : List α → Nat → α → α
-  | [],    i,   u => u
-  | a::as, 0,   u => a
-  | a::as, i+1, u => getIdx as i u
+def List.getIdx : (l : List α) → Fin l.length → α
+  | [],    ⟨_, i⟩ => by
+    simp [length] at i
+    apply absurd i
+    cases i
+  | a::as, ⟨0, _⟩ => a
+  | a::as, ⟨i+1, h⟩ => by
+    apply getIdx as ⟨i, _⟩
+    simp [List.length_cons] at h
+    apply Nat.lt_of_succ_lt_succ
+    assumption
 
 structure Context (α : Type u) where
   op    : α → α → α
-  unit  : α
   assoc : (a b c : α) → op (op a b) c = op a (op b c)
   comm  : (a b : α) → op a b = op b a
   vars  : List α
@@ -20,50 +26,50 @@ structure Context (α : Type u) where
 theorem Context.left_comm (ctx : Context α) (a b c : α) : ctx.op a (ctx.op b c) = ctx.op b (ctx.op a c) := by
   rw [← ctx.assoc, ctx.comm a b, ctx.assoc]
 
-def Expr.denote (ctx : Context α) : Expr → α
+def Expr.denote (ctx : Context α) : Expr ctx.vars.length → α
   | Expr.op a b => ctx.op (denote ctx a) (denote ctx b)
-  | Expr.var i  => ctx.vars.getIdx i ctx.unit
+  | Expr.var i  => ctx.vars.getIdx i
 
-theorem Expr.denote_op (ctx : Context α) (a b : Expr) : denote ctx (Expr.op a b) = ctx.op (denote ctx a) (denote ctx b) :=
+theorem Expr.denote_op (ctx : Context α) (a b : Expr ctx.vars.length) : denote ctx (Expr.op a b) = ctx.op (denote ctx a) (denote ctx b) :=
   rfl
 
-def Expr.concat : Expr → Expr → Expr
+def Expr.concat : Expr n → Expr n → Expr n
   | Expr.op a b, c => Expr.op a (concat b c)
   | Expr.var i, c  => Expr.op (Expr.var i) c
 
-theorem Expr.denote_concat (ctx : Context α) (a b : Expr) : denote ctx (concat a b) = denote ctx (Expr.op a b) := by
+theorem Expr.denote_concat (ctx : Context α) (a b : Expr ctx.vars.length) : denote ctx (concat a b) = denote ctx (Expr.op a b) := by
   induction a with
   | var i => rfl
   | op _ _ _ ih => simp [denote, ih, ctx.assoc]
 
-def Expr.flat : Expr → Expr
+def Expr.flat : Expr n → Expr n
   | Expr.op a b => concat (flat a) (flat b)
   | Expr.var i  => Expr.var i
 
-theorem Expr.denote_flat (ctx : Context α) (e : Expr) : denote ctx (flat e) = denote ctx e := by
+theorem Expr.denote_flat (ctx : Context α) (e : Expr ctx.vars.length) : denote ctx (flat e) = denote ctx e := by
   induction e with
   | var i => rfl
   | op a b ih₁ ih₂ => simp [flat, denote, denote_concat, ih₁, ih₂]
 
-theorem Expr.eq_of_flat (ctx : Context α) (a b : Expr) (h : flat a = flat b) : denote ctx a = denote ctx b := by
+theorem Expr.eq_of_flat (ctx : Context α) (a b : Expr ctx.vars.length) (h : flat a = flat b) : denote ctx a = denote ctx b := by
   have h := congrArg (denote ctx) h
   simp [denote_flat] at h
   assumption
 
-def Expr.length : Expr → Nat
+def Expr.length : Expr n → Nat
   | op a b => 1 + b.length
   | _      => 1
 
-def Expr.sort (e : Expr) : Expr :=
+def Expr.sort (e : Expr n) : Expr n :=
   loop e.length e
 where
-  loop : Nat → Expr → Expr
+  loop : Nat → Expr n → Expr n
     | fuel+1, Expr.op a e =>
       let (e₁, e₂) := swap a e
       Expr.op e₁ (loop fuel e₂)
     | _, e => e
 
-  swap : Expr → Expr → Expr × Expr
+  swap : Expr n → Expr n → Expr n × Expr n
     | Expr.var i, Expr.op (Expr.var j) e =>
       if i > j then
         let (e₁, e₂) := swap (Expr.var j) e
@@ -78,10 +84,10 @@ where
         (Expr.var i, Expr.var j)
     | e₁, e₂ => (e₁, e₂)
 
-theorem Expr.denote_sort (ctx : Context α) (e : Expr) : denote ctx (sort e) = denote ctx e := by
+theorem Expr.denote_sort (ctx : Context α) (e : Expr ctx.vars.length) : denote ctx (sort e) = denote ctx e := by
   apply denote_loop
 where
-  denote_loop (n : Nat) (e : Expr) : denote ctx (sort.loop n e) = denote ctx e := by
+  denote_loop (n : Nat) (e : Expr ctx.vars.length) : denote ctx (sort.loop n e) = denote ctx e := by
     induction n generalizing e with
     | zero => rfl
     | succ n ih =>
@@ -97,7 +103,7 @@ where
           simp [denote, ih]
           assumption
 
-  denote_swap (e₁ e₂ : Expr) : denote ctx (Expr.op (sort.swap e₁ e₂).1 (sort.swap e₁ e₂).2) = denote ctx (Expr.op e₁ e₂) := by
+  denote_swap (e₁ e₂ : Expr ctx.vars.length) : denote ctx (Expr.op (sort.swap e₁ e₂).1 (sort.swap e₁ e₂).2) = denote ctx (Expr.op e₁ e₂) := by
     induction e₂ generalizing e₁ with
     | op a b ih' ih =>
       clear ih'
@@ -128,7 +134,7 @@ where
         focus simp [sort.swap, h]
       | _ => rfl
 
-theorem Expr.eq_of_sort_flat (ctx : Context α) (a b : Expr) (h : sort (flat a) = sort (flat b)) : denote ctx a = denote ctx b := by
+theorem Expr.eq_of_sort_flat (ctx : Context α) (a b : Expr ctx.vars.length) (h : sort (flat a) = sort (flat b)) : denote ctx a = denote ctx b := by
   have h := congrArg (denote ctx) h
   simp [denote_flat, denote_sort] at h
   assumption
@@ -138,21 +144,19 @@ theorem ex₁ (x₁ x₂ x₃ x₄ : Nat) : (x₁ + x₂) + (x₃ + x₄) = x₁
     { op    := Nat.add
       assoc := Nat.add_assoc
       comm  := Nat.add_comm
-      unit  := Nat.zero
       vars  := [x₁, x₂, x₃, x₄] }
-    (Expr.op (Expr.op (Expr.var 0) (Expr.var 1)) (Expr.op (Expr.var 2) (Expr.var 3)))
-    (Expr.op (Expr.op (Expr.op (Expr.var 0) (Expr.var 1)) (Expr.var 2)) (Expr.var 3))
-    rfl
+    (Expr.op (Expr.op (Expr.var ⟨0, by simp⟩) (Expr.var ⟨1, by simp⟩)) (Expr.op (Expr.var ⟨2, by simp⟩) (Expr.var ⟨3, by simp⟩)))
+    (Expr.op (Expr.op (Expr.op (Expr.var ⟨0, by simp⟩) (Expr.var ⟨1, by simp⟩)) (Expr.var ⟨2, by simp⟩)) (Expr.var ⟨3, by simp⟩))
+    (by rfl)
 
 theorem ex₂ (x₁ x₂ x₃ x₄ : Nat) : (x₁ + x₂) + (x₃ + x₄) = x₃ + x₁ + x₂ + x₄ :=
   Expr.eq_of_sort_flat
     { op    := Nat.add
       assoc := Nat.add_assoc
       comm  := Nat.add_comm
-      unit  := Nat.zero
       vars  := [x₁, x₂, x₃, x₄] }
-    (Expr.op (Expr.op (Expr.var 0) (Expr.var 1)) (Expr.op (Expr.var 2) (Expr.var 3)))
-    (Expr.op (Expr.op (Expr.op (Expr.var 2) (Expr.var 0)) (Expr.var 1)) (Expr.var 3))
-    rfl
+    (Expr.op (Expr.op (Expr.var ⟨0, by simp⟩) (Expr.var ⟨1, by simp⟩)) (Expr.op (Expr.var ⟨2, by simp⟩) (Expr.var ⟨3, by simp⟩)))
+    (Expr.op (Expr.op (Expr.op (Expr.var ⟨2, by simp⟩) (Expr.var ⟨0, by simp⟩)) (Expr.var ⟨1, by simp⟩)) (Expr.var ⟨3, by simp⟩))
+    (by rfl)
 
 #print ex₂
